$$
\begin{align} 
(w^*, b^*) &= \mathop{\rm argmin} \limits_{(w, b)} \sum \limits_{i=1}^{m} (f(x_i)-y_i)^2 \\
&= \mathop{\rm argmin} \limits_{(w, b)} \sum \limits_{i=1}^{m} (wx_i+b-y_i)^2
\end{align}
$$

将上式展开：
$$
\begin{align}
\sum \limits_{i=1}^{m} (wx_i + b -y_i)^2 
&= \sum \limits_{i=1}^{m} [(wx_i+b)-y_i]^2 \\
&= \sum \limits_{i=1}^{m} [(wx_i +b)^2 + y_i^2 - 2(wx_i+b)y_i] \\
&= \sum \limits_{i=1}^{m} [w^2x_i^2 + b^2 + 2wx_ib + y_i^2 - 2wx_iy_i - 2by_i] \\
&= \sum \limits_{i=1}^{m} [x_i^2w^2 + 2(x_ib - x_iy_i)w + b^2 + y_i^2 -2by_i] \tag{1}\\
&= \sum \limits_{i=1}^{m} [b^2 + 2(wx_i - y_i)b + w^2x_i^2 + y_i^2 -2wx_iy_i] \tag{2}
\end{align}
$$
分别对$w$和$b$进行求导：
$$
\begin{align}
\frac{\partial L(w, b)}{\partial w} 
&= \frac{\partial L}{\partial w} \left[\sum \limits_{i=1}^{m}{(wx_i+b-y_i)^2} \right] \\
&= \sum \limits_{i=1}^{m} \frac{\partial L}{\partial w} (wx_i+b-y_i)^2 \\
&= \sum \limits_{i=1}^{m} 2(wx_i+b-y_i)x_i \\
&= \sum \limits_{i=1}^{m} 2(wx_i^2+bx_i-x_iy_i) \\
&= 2(w\sum \limits_{i=1}^{m}x_i^2+b\sum \limits_{i=1}^{m}x_i-\sum \limits_{i=1}^{m}x_iy_i) \\
\end{align}
$$
